systems/TreeStatic.v
@@ -1,0 +1,872 @@
+Require Import Verdi.
+Require Import HandlerMonad.
+Require Import NameOverlay.
+
+Require Import TotalMapSimulations.
+Require Import PartialMapSimulations.
+Require Import PartialExtendedMapSimulations.
+
+Require Import UpdateLemmas.
+Local Arguments update {_} {_} _ _ _ _ : simpl never.
+
+Require Import Sumbool.
+
+Require Import mathcomp.ssreflect.ssreflect.
+Require Import mathcomp.ssreflect.ssrbool.
+
+Require Import Orders.
+Require Import MSetFacts.
+Require Import MSetProperties.
+Require Import FMapInterface.
+
+Require Import Sorting.Permutation.
+
+Require Import FailureRecorderStatic.
+
+Set Implicit Arguments.
+
+Module Tree (Import NT : NameType)  
+ (NOT : NameOrderedType NT) (NSet : MSetInterface.S with Module E := NOT) 
+ (NOTC : NameOrderedTypeCompat NT) (NMap : FMapInterface.S with Module E := NOTC)
+ (Import RNT : RootNameType NT) (Import ANT : AdjacentNameType NT).
+
+Module A := Adjacency NT NOT NSet ANT.
+Import A.
+
+Module FR := FailureRecorder NT NOT NSet ANT.
+
+Module NSetFacts := Facts NSet.
+Module NSetProps := Properties NSet.
+Module NSetOrdProps := OrdProperties NSet.
+
+Definition lv := nat.
+Definition lv_eq_dec := Nat.eq_dec.
+
+Inductive Msg : Set := 
+| Fail : Msg
+| Level : option lv -> Msg.
+
+Definition Msg_eq_dec : forall x y : Msg, {x = y} + {x <> y}.
+decide equality.
+case: o; case: o0.
+- move => n m.
+  case (lv_eq_dec n m) => H_dec; first by rewrite H_dec; left.
+  right.
+  move => H_eq.
+  injection H_eq => H_eq'.
+  by rewrite H_eq' in H_dec.
+- by right.
+- by right.
+- by left.
+Defined.
+
+Inductive Input : Set :=
+| LevelRequest : Input
+| Broadcast : Input.
+
+Definition Input_eq_dec : forall x y : Input, {x = y} + {x <> y}.
+decide equality.
+Defined.
+
+Inductive Output : Set :=
+| LevelResponse : option lv -> Output.
+
+Definition Output_eq_dec : forall x y : Output, {x = y} + {x <> y}.
+decide equality.
+case: o; case: o0.
+- move => n m.
+  case (lv_eq_dec n m) => H_dec; first by rewrite H_dec; left.
+  right.
+  move => H_eq.
+  injection H_eq => H_eq'.
+  by rewrite H_eq' in H_dec.
+- by right.
+- by right.
+- by left.
+Defined.
+
+Definition NL := NMap.t lv.
+
+Record Data := mkData { 
+  adjacent : NS ; 
+  broadcast : bool ; 
+  levels : NL
+}.
+
+Definition InitData (n : name) := 
+if root_dec n then
+  {| adjacent := adjacency n nodes ;
+     broadcast := true ;
+     levels := NMap.empty lv |}
+else
+  {| adjacent := adjacency n nodes ;
+     broadcast := false ;
+     levels := NMap.empty lv |}.
+
+Inductive level_in (fs : NS) (fl : NL) (n : name) (lv' : lv) : Prop :=
+| in_level_in : NSet.In n fs -> NMap.find n fl = Some lv' -> level_in fs fl n lv'.
+
+Inductive min_level (fs : NS) (fl : NL) (n : name) (lv' : lv) : Prop :=
+| min_lv_min : level_in fs fl n lv' -> 
+  (forall (lv'' : lv) (n' : name), level_in fs fl n' lv'' -> ~ lv'' < lv') ->
+  min_level fs fl n lv'.
+
+Record st_par := mk_st_par { st_par_set : NS ; st_par_map : NL }.
+
+Record nlv := mk_nlv { nlv_n : name ; nlv_lv : lv }.
+
+Definition st_par_lt (s s' : st_par) : Prop :=
+NSet.cardinal s.(st_par_set) < NSet.cardinal s'.(st_par_set).
+
+Lemma st_par_lt_well_founded : well_founded st_par_lt.
+Proof.
+apply (well_founded_lt_compat _ (fun s => NSet.cardinal s.(st_par_set))).
+by move => x y; rewrite /st_par_lt => H.
+Qed.
+
+Definition par_t (s : st_par) := 
+{ nlv' | min_level s.(st_par_set) s.(st_par_map) nlv'.(nlv_n) nlv'.(nlv_lv) }+
+{ ~ exists nlv', level_in s.(st_par_set) s.(st_par_map) nlv'.(nlv_n) nlv'.(nlv_lv) }.
+
+Definition par_F : forall s : st_par, 
+  (forall s' : st_par, st_par_lt s' s -> par_t s') ->
+  par_t s.
+rewrite /par_t.
+refine 
+  (fun (s : st_par) par_rec => 
+   match NSet.choose s.(st_par_set) as sopt return (_ = sopt -> _) with
+   | Some n => fun (H_eq : _) => 
+     match par_rec (mk_st_par (NSet.remove n s.(st_par_set)) s.(st_par_map)) _ with
+     | inleft (exist nlv' H_min) =>
+       match NMap.find n s.(st_par_map) as n' return (_ = n' -> _) with
+       | Some lv' => fun (H_find : _) => 
+         match lt_dec lv' nlv'.(nlv_lv)  with
+         | left H_dec => inleft _ (exist _ (mk_nlv n lv') _)
+         | right H_dec => inleft _ (exist _ nlv' _)
+         end
+       | None => fun (H_find : _) => inleft _ (exist _ nlv' _)
+       end (refl_equal _)
+     | inright H_min =>
+       match NMap.find n s.(st_par_map) as n' return (_ = n' -> _) with
+       | Some lv' => fun (H_find : _) => inleft _ (exist _ (mk_nlv n lv') _)
+       | None => fun (H_find : _) => inright _ _
+       end (refl_equal _)
+     end
+   | None => fun (H_eq : _) => inright _ _
+   end (refl_equal _)) => /=.
+- rewrite /st_par_lt /=.
+  apply NSet.choose_spec1 in H_eq.
+  set sr := NSet.remove _ _.
+  have H_notin: ~ NSet.In n sr by move => H_in; apply NSetFacts.remove_1 in H_in.
+  have H_add: NSetProps.Add n sr s.(st_par_set).
+    rewrite /NSetProps.Add.
+    move => n'.
+    split => H_in.
+      case (name_eq_dec n n') => H_eq'; first by left.
+      by right; apply NSetFacts.remove_2.
+    case: H_in => H_in; first by rewrite -H_in.
+    by apply NSetFacts.remove_3 in H_in.
+  have H_card := NSetProps.cardinal_2 H_notin H_add.
+  rewrite H_card {H_notin H_add H_card}.
+  by auto with arith.
+- apply NSet.choose_spec1 in H_eq.
+  rewrite /= {s0} in H_min.
+  apply min_lv_min; first exact: in_level_in.
+  move => lv'' n' H_lv.
+  inversion H_lv => {H_lv}.
+  inversion H_min => {H_min}.
+  case (name_eq_dec n n') => H_eq'.
+    rewrite -H_eq' in H0.
+    rewrite H_find in H0.
+    injection H0 => H_eq_lt.
+    rewrite H_eq_lt.
+    by auto with arith.
+  suff H_suff: ~ lv'' < nlv'.(nlv_lv) by omega.
+  apply: (H2 _ n').
+  apply: in_level_in => //.
+  by apply NSetFacts.remove_2.
+- apply NSet.choose_spec1 in H_eq.
+  rewrite /= {s0} in H_min.
+  inversion H_min => {H_min}.
+  inversion H => {H}.
+  apply min_lv_min.
+    apply: in_level_in => //.
+    by apply NSetFacts.remove_3 in H1.
+  move => lv'' n' H_lv.
+  inversion H_lv => {H_lv}.
+  case (name_eq_dec n n') => H_eq'.
+    rewrite -H_eq' in H3.
+    rewrite H_find in H3.
+    injection H3 => H_eq_lv.
+    by rewrite -H_eq_lv.
+  apply: (H0 _ n').
+  apply: in_level_in => //.
+  exact: NSetFacts.remove_2.
+- apply NSet.choose_spec1 in H_eq.
+  rewrite /= {s0} in H_min.
+  inversion H_min => {H_min}.
+  inversion H => {H}.
+  apply min_lv_min.
+    apply: in_level_in => //.
+    by apply NSetFacts.remove_3 in H1.
+  move => lv' n' H_lv.
+  inversion H_lv => {H_lv}.
+  case (name_eq_dec n n') => H_eq'.
+    rewrite -H_eq' in H3.
+    by rewrite H_find in H3.
+  apply: (H0 _ n').
+  apply: in_level_in => //.
+  exact: NSetFacts.remove_2.
+- apply NSet.choose_spec1 in H_eq.
+  rewrite /= in H_min.
+  apply min_lv_min; first exact: in_level_in.
+  move => lv'' n' H_lv.
+  inversion H_lv.
+  case (name_eq_dec n n') => H_eq'.
+    rewrite -H_eq' in H0.
+    rewrite H_find in H0.
+    injection H0 => H_eq_lv.
+    rewrite H_eq_lv.  
+    by auto with arith.
+  move => H_lt.
+  case: H_min.
+  exists (mk_nlv n' lv'') => /=.
+  apply: in_level_in => //.
+  exact: NSetFacts.remove_2.
+- apply NSet.choose_spec1 in H_eq.
+  rewrite /= in H_min.
+  move => [nlv' H_lv].
+  inversion H_lv => {H_lv}.
+  case: H_min.
+  exists nlv'.
+  case (name_eq_dec n nlv'.(nlv_n)) => H_eq'.
+    rewrite -H_eq' in H0.
+    by rewrite H_find in H0.
+  apply: in_level_in => //.
+  exact: NSetFacts.remove_2.
+- apply NSet.choose_spec2 in H_eq.
+  move => [nlv' H_lv].
+  inversion H_lv => {H_lv}.
+  by case (H_eq nlv'.(nlv_n)).
+Defined.
+
+Definition par : forall (s : st_par), par_t s :=
+  @well_founded_induction_type
+  st_par
+  st_par_lt
+  st_par_lt_well_founded
+  par_t
+  par_F.
+
+Definition lev : forall (s : st_par),
+{ lv' | exists n, exists lv'', min_level s.(st_par_set) s.(st_par_map) n lv'' /\ lv' = lv'' + 1%nat }+
+{ ~ exists n, exists lv', level_in s.(st_par_set) s.(st_par_map) n lv' }.
+refine
+  (fun (s : st_par) =>
+   match par s with
+   | inleft (exist nlv' H_min) => inleft _ (exist _ (1 + nlv'.(nlv_lv)) _)
+   | inright H_ex => inright _ _
+   end).
+- rewrite /= in H_min.
+  exists nlv'.(nlv_n); exists nlv'.(nlv_lv); split => //.
+  by omega.
+- move => [n [lv' H_lv] ].
+  case: H_ex => /=.
+  by exists (mk_nlv n lv').
+Defined.
+
+Definition parent (fs : NS) (fl : NL) : option name :=
+match par (mk_st_par fs fl) with
+| inleft (exist nlv' _) => Some nlv'.(nlv_n)
+| inright _ => None
+end.
+
+Definition level (fs : NS) (fl : NL) : option lv :=
+match lev (mk_st_par fs fl) with
+| inleft (exist lv' _) => Some lv'
+| inright _ => None
+end.
+
+Definition olv_eq_dec : forall (lvo lvo' : option lv), { lvo = lvo' }+{ lvo <> lvo' }.
+decide equality.
+exact: lv_eq_dec.
+Defined.
+
+Definition Handler (S : Type) := GenHandler (name * Msg) S Output unit.
+
+Definition RootNetHandler (src : name) (msg : Msg) : Handler Data :=
+st <- get ;;
+match msg with 
+| Level _ => nop 
+| Fail => 
+  put {| adjacent := NSet.remove src st.(adjacent) ;
+         broadcast := st.(broadcast) ;
+         levels := st.(levels) |}
+end.
+
+Definition NonRootNetHandler (me src: name) (msg : Msg) : Handler Data :=
+st <- get ;;
+match msg with
+| Level None =>
+  if olv_eq_dec (level st.(adjacent) st.(levels)) (level st.(adjacent) (NMap.remove src st.(levels))) then
+    put {| adjacent := st.(adjacent) ;           
+           broadcast := st.(broadcast) ;
+           levels := NMap.remove src st.(levels) |}
+  else 
+    put {| adjacent := st.(adjacent) ;           
+           broadcast := true ;
+           levels := NMap.remove src st.(levels) |}
+| Level (Some lv') =>
+  if olv_eq_dec (level st.(adjacent) st.(levels)) (level st.(adjacent) (NMap.add src lv' st.(levels))) then
+    put {| adjacent := st.(adjacent) ;
+           broadcast := st.(broadcast) ;
+           levels := NMap.add src lv' st.(levels) |}
+  else
+    put {| adjacent := st.(adjacent) ;
+           broadcast := true ;
+           levels := NMap.add src lv' st.(levels) |}
+| Fail => 
+  if olv_eq_dec (level st.(adjacent) st.(levels)) (level (NSet.remove src st.(adjacent)) (NMap.remove src st.(levels))) then
+    put {| adjacent := NSet.remove src st.(adjacent) ;
+           broadcast := st.(broadcast) ;
+           levels := NMap.remove src st.(levels) |}
+  else
+    put {| adjacent := NSet.remove src st.(adjacent) ;
+           broadcast := true ;
+           levels := NMap.remove src st.(levels) |}
+end.
+
+Definition NetHandler (me src : name) (msg : Msg) : Handler Data :=
+if root_dec me then RootNetHandler src msg 
+else NonRootNetHandler me src msg.
+
+Definition level_fold (lvo : option lv) (n : name) (partial : list (name * Msg)) : list (name * Msg) :=
+(n, Level lvo) :: partial.
+
+Definition level_adjacent (lvo : option lv) (fs : NS) : list (name * Msg) :=
+NSet.fold (level_fold lvo) fs [].
+
+Definition send_level_fold (lvo : option lv) (n : name) (res : Handler Data) : Handler Data :=
+send (n, Level lvo) ;; res.
+
+Definition send_level_adjacent (lvo : option lv) (fs : NS) : Handler Data :=
+NSet.fold (send_level_fold lvo) fs nop.
+
+Definition RootIOHandler (i : Input) : Handler Data :=
+st <- get ;;
+match i with
+| Broadcast => 
+  when st.(broadcast)
+  (send_level_adjacent (Some 0) st.(adjacent) ;;
+   put {| adjacent := st.(adjacent);
+          broadcast := false;
+          levels := st.(levels) |})
+| LevelRequest => 
+  write_output (LevelResponse (Some 0))
+end.
+
+Definition NonRootIOHandler (i : Input) : Handler Data :=
+st <- get ;;
+match i with
+| Broadcast =>
+  when st.(broadcast)
+  (send_level_adjacent (level st.(adjacent) st.(levels)) st.(adjacent) ;; 
+  put {| adjacent := st.(adjacent);
+         broadcast := false;
+         levels := st.(levels) |})
+| LevelRequest =>   
+  write_output (LevelResponse (level st.(adjacent) st.(levels)))
+end.
+
+Definition IOHandler (me : name) (i : Input) : Handler Data :=
+if root_dec me then RootIOHandler i 
+else NonRootIOHandler i.
+
+Instance Tree_BaseParams : BaseParams :=
+  {
+    data := Data;
+    input := Input;
+    output := Output
+  }.
+
+Instance Tree_MultiParams : MultiParams Tree_BaseParams NT_NameParams :=
+  {
+    msg  := Msg ;
+    msg_eq_dec := Msg_eq_dec ;
+    init_handlers := InitData ;
+    net_handlers := fun dst src msg s =>
+                      runGenHandler_ignore s (NetHandler dst src msg) ;
+    input_handlers := fun nm msg s =>
+                        runGenHandler_ignore s (IOHandler nm msg)
+  }.
+
+Instance Tree_FailMsgParams : FailMsgParams Tree_MultiParams :=
+  {
+    msg_fail := Fail
+  }.
+
+Lemma net_handlers_NetHandler :
+  forall dst src m st os st' ms,
+    net_handlers dst src m st = (os, st', ms) ->
+    NetHandler dst src m st = (tt, os, st', ms).
+Proof.
+intros.
+simpl in *.
+monad_unfold.
+repeat break_let.
+find_inversion.
+destruct u. auto.
+Qed.
+
+Lemma NetHandler_cases : 
+  forall dst src msg st out st' ms,
+    NetHandler dst src msg st = (tt, out, st', ms) ->
+    (root dst /\ msg = Fail /\ 
+     st'.(adjacent) = NSet.remove src st.(adjacent) /\
+     st'.(broadcast) = st.(broadcast) /\
+     st'.(levels) = st.(levels) /\
+     out = [] /\ ms = []) \/
+    (~ root dst /\ msg = Fail /\ 
+     level st.(adjacent) st.(levels) = level (NSet.remove src st.(adjacent)) (NMap.remove src st.(levels)) /\
+     st'.(adjacent) = NSet.remove src st.(adjacent) /\
+     st'.(broadcast) = st.(broadcast) /\
+     st'.(levels) = NMap.remove src st.(levels) /\
+     out = [] /\ ms = []) \/
+    (~ root dst /\ msg = Fail /\ 
+     level st.(adjacent) st.(levels) <> level (NSet.remove src st.(adjacent)) (NMap.remove src st.(levels)) /\
+     st'.(adjacent) = NSet.remove src st.(adjacent) /\
+     st'.(broadcast) = true /\
+     st'.(levels) = NMap.remove src st.(levels) /\
+     out = [] /\ ms = []) \/
+    (root dst /\ exists lvo, msg = Level lvo /\ 
+     st' = st /\
+     out = [] /\ ms = []) \/
+    (~ root dst /\ exists lv_msg, msg = Level (Some lv_msg) /\
+     level st.(adjacent) st.(levels) = level st.(adjacent) (NMap.add src lv_msg st.(levels)) /\
+     st'.(adjacent) = st.(adjacent) /\
+     st'.(broadcast) = st.(broadcast) /\
+     st'.(levels) = NMap.add src lv_msg st.(levels) /\
+     out = [] /\ ms = []) \/
+    (~ root dst /\ exists lv_msg, msg = Level (Some lv_msg) /\
+     level st.(adjacent) st.(levels) <> level st.(adjacent) (NMap.add src lv_msg st.(levels)) /\
+     st'.(adjacent) = st.(adjacent) /\
+     st'.(broadcast) = true /\
+     st'.(levels) = NMap.add src lv_msg st.(levels) /\
+     out = [] /\ ms = []) \/
+    (~ root dst /\ msg = Level None /\
+     level st.(adjacent) st.(levels) = level st.(adjacent) (NMap.remove src st.(levels)) /\
+     st'.(adjacent) = st.(adjacent) /\
+     st'.(broadcast) = st.(broadcast) /\
+     st'.(levels) = NMap.remove src st.(levels) /\
+     out = [] /\ ms = []) \/
+    (~ root dst /\ msg = Level None /\
+     level st.(adjacent) st.(levels) <> level st.(adjacent) (NMap.remove src st.(levels)) /\
+     st'.(adjacent) = st.(adjacent) /\
+     st'.(broadcast) = true /\
+     st'.(levels) = NMap.remove src st.(levels) /\
+     out = [] /\ ms = []).
+Proof.
+move => dst src msg st out st' ms.
+rewrite /NetHandler /RootNetHandler /NonRootNetHandler.
+case: msg; monad_unfold.
+- case root_dec => /= H_dec.
+  * move => H_eq.
+    injection H_eq => H_ms H_st H_out; rewrite -H_st /=.
+    by left.
+  * case olv_eq_dec => /= H_dec' H_eq; injection H_eq => H_ms H_st H_out; rewrite -H_st /=.
+      by right; left.
+    by right; right; left.
+- case root_dec => /= H_dec olv_msg.
+    move => H_eq.
+    injection H_eq => H_ms H_st H_out; rewrite -H_st /=.
+    right; right; right; left.
+    split => //.
+    by exists olv_msg.
+  case H_olv_dec: olv_msg => [lv_msg|]; case olv_eq_dec => /= H_dec' H_eq; injection H_eq => H_ms H_st H_out; rewrite -H_st /=.
+  * right; right; right; right; left.
+    split => //.
+    by exists lv_msg.
+  * right; right; right; right; right; left.
+    split => //.
+    by exists lv_msg.
+  * by right; right; right; right; right; right; left.
+  * by right; right; right; right; right; right; right.
+Qed.
+
+Lemma input_handlers_IOHandler :
+  forall h i d os d' ms,
+    input_handlers h i d = (os, d', ms) ->
+    IOHandler h i d = (tt, os, d', ms).
+Proof.
+intros.
+simpl in *.
+monad_unfold.
+repeat break_let.
+find_inversion.
+destruct u. auto.
+Qed.
+
+Lemma fold_left_level_fold_eq :
+forall ns nml olv,
+fold_left (fun l n => level_fold olv n l) ns nml = fold_left (fun l n => level_fold olv n l) ns [] ++ nml.
+Proof.
+elim => //=.
+move => n ns IH nml olv.
+rewrite /level_fold /=.
+rewrite IH.
+have IH' := IH ([(n, Level olv)]).
+rewrite IH'.
+set bla := fold_left _ _ _.
+rewrite -app_assoc.
+by rewrite app_assoc.
+Qed.
+
+Lemma send_level_fold_app :
+  forall ns st olv nm,
+snd (fold_left 
+       (fun (a : Handler Data) (e : NSet.elt) => send_level_fold olv e a) ns
+       (fun s : Data => (tt, [], s, nm)) st) = 
+snd (fold_left 
+       (fun (a : Handler Data) (e : NSet.elt) => send_level_fold olv e a) ns
+       (fun s : Data => (tt, [], s, [])) st) ++ nm.
+Proof.
+elim => //=.
+move => n ns IH st olv nm.
+rewrite {1}/send_level_fold /=.
+monad_unfold.
+rewrite /=.
+rewrite IH.
+rewrite app_assoc.
+by rewrite -IH.
+Qed.
+
+Lemma send_level_adjacent_fst_eq : 
+forall fs olv st,
+  snd (send_level_adjacent olv fs st) = level_adjacent olv fs.
+Proof.
+move => fs olv st.
+rewrite /send_level_adjacent /level_adjacent.
+rewrite 2!NSet.fold_spec.
+move: olv st.
+elim: NSet.elements => [|n ns IH] //=.
+move => olv st.
+rewrite {2}/level_fold {2}/send_level_fold.
+rewrite fold_left_level_fold_eq.
+have IH' := IH olv st.
+rewrite -IH'.
+monad_unfold.
+by rewrite -send_level_fold_app.
+Qed.
+
+Lemma fst_fst_fst_tt_send_level_fold : 
+forall ns nm olv st,
+fst
+  (fst
+     (fst
+        (fold_left
+           (fun (a : Handler Data) (e : NSet.elt) =>
+              send_level_fold olv e a) ns
+           (fun s : Data => (tt, [], s, nm)) st))) = tt.
+Proof.
+elim => //=.
+move => n ns IH nm olv st.
+by rewrite IH.
+Qed.
+
+Lemma send_level_adjacent_fst_fst_eq : 
+forall fs olv st,
+  fst (fst (fst (send_level_adjacent olv fs st))) = tt.
+Proof.
+move => fs olv st.
+rewrite /send_level_adjacent.
+rewrite NSet.fold_spec.
+by rewrite fst_fst_fst_tt_send_level_fold.
+Qed.
+
+Lemma snd_fst_fst_out_send_level_fold : 
+forall ns nm olv st,
+snd
+  (fst
+     (fst
+        (fold_left
+           (fun (a : Handler Data) (e : NSet.elt) =>
+              send_level_fold olv e a) ns
+           (fun s : Data => (tt, [], s, nm)) st))) = [].
+Proof.
+elim => //=.
+move => n ns IH nm olv st.
+by rewrite IH.
+Qed.
+
+Lemma snd_fst_st_send_level_fold : 
+forall ns nm olv st,
+snd (fst
+        (fold_left
+           (fun (a : Handler Data) (e : NSet.elt) =>
+              send_level_fold olv e a) ns
+           (fun s : Data => (tt, [], s, nm)) st)) = st.
+Proof.
+elim => //=.
+move => n ns IH nm olv st.
+by rewrite IH.
+Qed.
+
+Lemma send_level_adjacent_snd_fst_fst : 
+forall fs olv st,
+  snd (fst (fst (send_level_adjacent olv fs st))) = [].
+Proof.
+move => fs olv st.
+rewrite /send_level_adjacent.
+rewrite NSet.fold_spec.
+by rewrite snd_fst_fst_out_send_level_fold.
+Qed.
+
+Lemma send_level_adjacent_snd_fst : 
+forall fs olv st,
+  snd (fst (send_level_adjacent olv fs st)) = st.
+Proof.
+move => fs olv st.
+rewrite /send_level_adjacent.
+rewrite NSet.fold_spec.
+by rewrite snd_fst_st_send_level_fold.
+Qed.
+
+Lemma send_level_adjacent_eq : 
+  forall fs olv st,
+  send_level_adjacent olv fs st = (tt, [], st, level_adjacent olv fs).
+Proof.
+move => fs olv st.
+case H_eq: send_level_adjacent => [[[u o] s b]].
+have H_eq'_1 := send_level_adjacent_fst_fst_eq fs olv st.
+rewrite H_eq /= in H_eq'_1.
+have H_eq'_2 := send_level_adjacent_fst_eq fs olv st.
+rewrite H_eq /= in H_eq'_2.
+have H_eq'_3 := send_level_adjacent_snd_fst_fst fs olv st.
+rewrite H_eq /= in H_eq'_3.
+have H_eq'_4 := send_level_adjacent_snd_fst fs olv st.
+rewrite H_eq /= in H_eq'_4.
+by rewrite H_eq'_1 H_eq'_2 H_eq'_3 H_eq'_4.
+Qed.
+
+Lemma IOHandler_cases :
+  forall h i st u out st' ms,
+      IOHandler h i st = (u, out, st', ms) ->
+      (root h /\ i = Broadcast /\ st.(broadcast) = true /\
+       st'.(adjacent) = st.(adjacent) /\
+       st'.(broadcast) = false /\
+       st'.(levels) = st.(levels) /\
+       out = [] /\ ms = level_adjacent (Some 0) st.(adjacent)) \/
+      (~ root h /\ i = Broadcast /\ st.(broadcast) = true /\
+       st'.(adjacent) = st.(adjacent) /\
+       st'.(broadcast) = false /\
+       st'.(levels) = st.(levels) /\
+       out = [] /\ ms = level_adjacent (level st.(adjacent) st.(levels)) st.(adjacent)) \/
+      (i = Broadcast /\ st.(broadcast) = false /\
+       st' = st /\
+       out = [] /\ ms = []) \/
+      (root h /\ i = LevelRequest /\
+       st' = st /\
+       out = [LevelResponse (Some 0)] /\ ms = []) \/
+      (~ root h /\ i = LevelRequest /\
+       st' = st /\
+       out = [LevelResponse (level st.(adjacent) st.(levels))] /\ ms = []).
+Proof.
+move => h i st u out st' ms.
+rewrite /IOHandler /RootIOHandler /NonRootIOHandler.
+case: i => [|]; monad_unfold.
+- case root_dec => /= H_dec H_eq; injection H_eq => H_ms H_st H_out H_tt; rewrite -H_st /=.
+    by right; right; right; left.
+  by right; right; right; right.
+- case root_dec => /= H_dec; case H_b: broadcast => /=.
+  * left.
+    repeat break_let.
+    injection Heqp => H_ms H_st H_out H_tt.
+    subst.
+    injection Heqp2 => H_ms H_st H_out H_tt.
+    subst.
+    injection H => H_ms H_st H_out H_tt.
+    subst.
+    rewrite /=.
+    have H_eq := send_level_adjacent_eq st.(adjacent) (Some 0) st.
+    rewrite Heqp5 in H_eq.
+    injection H_eq => H_eq_ms H_eq_st H_eq_o H_eq_tt.
+    rewrite H_eq_ms H_eq_o.
+    by rewrite app_nil_l -2!app_nil_end.
+  * right; right; left.
+    injection H => H_ms H_st H_o H_tt.
+    by rewrite H_st H_o H_ms.
+  * right; left.
+    repeat break_let.
+    injection Heqp => H_ms H_st H_out H_tt.
+    subst.
+    injection Heqp2 => H_ms H_st H_out H_tt.
+    subst.
+    injection H => H_ms H_st H_out H_tt.
+    subst.
+    rewrite /=.
+    have H_eq := send_level_adjacent_eq st.(adjacent) (level st.(adjacent) st.(levels)) st.
+    rewrite Heqp5 in H_eq.
+    injection H_eq => H_eq_ms H_eq_st H_eq_o H_eq_tt.
+    rewrite H_eq_ms H_eq_o.
+    by rewrite app_nil_l -2!app_nil_end.
+  * right; right; left.
+    injection H => H_ms H_st H_o H_tt.
+    by rewrite H_st H_o H_ms.
+Qed.
+
+Ltac net_handler_cases := 
+  find_apply_lem_hyp NetHandler_cases; 
+  intuition idtac; try break_exists; 
+  intuition idtac; subst; 
+  repeat find_rewrite.
+
+Ltac io_handler_cases := 
+  find_apply_lem_hyp IOHandler_cases; 
+  intuition idtac; try break_exists; 
+  intuition idtac; subst; 
+  repeat find_rewrite.
+
+Instance Tree_FailureRecorder_base_params_pt_map : BaseParamsPartialMap Tree_BaseParams FR.FailureRecorder_BaseParams :=
+  {
+    pt_map_data := fun d => FR.mkData d.(adjacent) ;
+    pt_map_input := fun _ => None ;
+    pt_map_output := fun _ => None
+  }.
+
+Instance Tree_FailureRecorder_name_params_tot_map : NameParamsTotalMap NT_NameParams FR.A.NT_NameParams :=
+  {
+    tot_map_name := id ;
+    tot_map_name_inv := id
+  }.
+
+Instance Tree_FailureRecorder_multi_params_pt_map : MultiParamsPartialMap Tree_FailureRecorder_base_params_pt_map Tree_FailureRecorder_name_params_tot_map Tree_MultiParams FR.FailureRecorder_MultiParams :=
+  {
+    pt_map_msg := fun m => match m with Fail => Some FR.Fail | _ => None end ;
+  }.
+
+Lemma tot_map_name_inv_inverse : forall n, tot_map_name_inv (tot_map_name n) = n.
+Proof. by []. Qed.
+
+Lemma tot_map_name_inverse_inv : forall n, tot_map_name (tot_map_name_inv n) = n.
+Proof. by []. Qed.
+
+Lemma pt_init_handlers_eq : forall n,
+  pt_map_data (init_handlers n) = init_handlers (tot_map_name n).
+Proof.
+move => n.
+rewrite /= /InitData /=.
+by case root_dec => /= H_dec.
+Qed.
+
+Lemma pt_net_handlers_some : forall me src m st m',
+  pt_map_msg m = Some m' ->
+  pt_mapped_net_handlers me src m st = net_handlers (tot_map_name me) (tot_map_name src) m' (pt_map_data st).
+Proof.
+move => me src.
+case => // d.
+case => H_eq.
+rewrite /pt_mapped_net_handlers.
+repeat break_let.
+apply net_handlers_NetHandler in Heqp.
+net_handler_cases => //.
+- by rewrite /= /runGenHandler_ignore /= H1.
+- by rewrite /= /runGenHandler_ignore /id /= H2.
+- by rewrite /= /runGenHandler_ignore /id /= H2.
+Qed.
+
+Lemma pt_net_handlers_none : forall me src m st out st' ps,    
+  pt_map_msg m = None ->
+  net_handlers me src m st = (out, st', ps) ->
+  pt_map_data st' = pt_map_data st /\ pt_map_name_msgs ps = [] /\ pt_map_outputs out = [].
+Proof.
+move => me src.
+case => //.
+move => olv d out d' ps H_eq H_eq'.
+apply net_handlers_NetHandler in H_eq'.
+net_handler_cases => //.
+- case: d' H2 H3 H4 => /= adjacent0 broadcast0 levels0 H_eq' H_eq'' H_add.
+  by rewrite H_eq'.
+- case: d' H2 H3 H4 => /= adjacent0 broadcast0 levels0 H_eq' H_eq'' H_add.
+  by rewrite H_eq'.
+- case: d' H2 H3 H4 => /= adjacent0 broadcast0 levels0 H_eq' H_eq'' H_add.
+  by rewrite H_eq'.
+- case: d' H2 H3 H4 => /= adjacent0 broadcast0 levels0 H_eq' H_eq'' H_add.
+  by rewrite H_eq'.
+Qed.
+
+Lemma pt_input_handlers_some : forall me inp st inp',
+  pt_map_input inp = Some inp' ->
+  pt_mapped_input_handlers me inp st = input_handlers (tot_map_name me) inp' (pt_map_data st).
+Proof. by []. Qed.
+
+Lemma pt_input_handlers_none : forall me inp st out st' ps,
+  pt_map_input inp = None ->
+  input_handlers me inp st = (out, st', ps) ->
+  pt_map_data st' = pt_map_data st /\ pt_map_name_msgs ps = [] /\ pt_map_outputs out = [].
+Proof.
+move => me.
+case.
+- move => d out d' ps H_eq H_inp.
+  apply input_handlers_IOHandler in H_inp.
+  by io_handler_cases.
+- move => d out d' ps H_eq H_inp.
+  apply input_handlers_IOHandler in H_inp.
+  io_handler_cases => //.
+  * case: d' H2 H3 H4 => /= adjacent0 broadcast0 levels0 H_eq' H_eq'' H_eq_l.
+    by rewrite H_eq'.
+  * rewrite /level_adjacent NSet.fold_spec /flip /=.
+    elim: NSet.elements => //=.
+    move => n l IH.
+    rewrite /flip /= /level_fold.
+    rewrite fold_left_level_fold_eq.
+    by rewrite pt_map_name_msgs_app_distr /= IH.
+  * case: d' H2 H3 H4 => /= adjacent0 broadcast0 levels0 H_eq' H_eq'' H_eq_l.
+    by rewrite H_eq'.
+ * rewrite /level_adjacent NSet.fold_spec /flip /=.
+    elim: NSet.elements => //=.
+    move => n l IH.
+    rewrite /flip /= /level_fold.
+    rewrite fold_left_level_fold_eq.
+    by rewrite pt_map_name_msgs_app_distr /= IH.
+Qed.
+
+Lemma fail_msg_fst_snd : pt_map_msg msg_fail = Some (msg_fail).
+Proof. by []. Qed.
+
+Lemma adjacent_to_fst_snd : 
+  forall n n', adjacent_to n n' <-> adjacent_to (tot_map_name n) (tot_map_name n').
+Proof. by []. Qed.
+
+Theorem Tree_Failed_pt_mapped_simulation_star_1 :
+forall net failed tr,
+    @step_o_f_star _ _ _ _ Tree_FailMsgParams step_o_f_init (failed, net) tr ->
+    exists tr', @step_o_f_star _ _ _ _ FR.FailureRecorder_FailMsgParams step_o_f_init (failed, pt_map_onet net) tr' /\
+    pt_trace_remove_empty_out (pt_map_trace tr) = pt_trace_remove_empty_out tr'.
+Proof.
+have H_sim := @step_o_f_pt_mapped_simulation_star_1 _ _ _  _ _ _ _ _ _ tot_map_name_inv_inverse tot_map_name_inverse_inv pt_init_handlers_eq pt_net_handlers_some pt_net_handlers_none pt_input_handlers_some pt_input_handlers_none ANT_NameOverlayParams FR.A.ANT_NameOverlayParams adjacent_to_fst_snd _ _ fail_msg_fst_snd.
+rewrite /tot_map_name /= /id in H_sim.
+move => onet failed tr H_st.
+apply H_sim in H_st.
+move: H_st => [tr' [H_st H_eq]].
+rewrite map_id in H_st.
+by exists tr'.
+Qed.
+
+End Tree.
+
+(*
+Require Import StructTact.Fin.
+
+Module N3 : NatValue. Definition n := 3. End N3.
+Module FN_N3 : FinNameType N3 := FinName N3.
+Module NOT_N3 : NameOrderedType FN_N3 := FinNameOrderedType N3 FN_N3.
+Module NOTC_N3 : NameOrderedTypeCompat FN_N3 := FinNameOrderedTypeCompat N3 FN_N3.
+Module ANC_N3 := FinCompleteAdjacentNameType N3 FN_N3.
+Require Import MSetList.
+Module N3Set <: MSetInterface.S := MSetList.Make NOT_N3.
+Require Import FMapList.
+Module N3Map <: FMapInterface.S := FMapList.Make NOTC_N3.
+Module RNT_N3 := FinRootNameType N3 FN_N3.
+Module T := Tree FN_N3 NOT_N3 N3Set NOTC_N3 N3Map RNT_N3 ANC_N3.
+Print T.Msg.
+*)
